src/coq/CompilerProp.v
@@ -17,18 +17,26 @@ Require Import ZArith String Omega List Equalities MSets.
 Import ListNotations.
 
 (* Vellvm dependencies *)
-Require Import Vellvm.Ollvm_ast Vellvm.Compiler Vellvm.AstLib Vellvm.CFG Vellvm.StepSemantics Vellvm.Memory.
+Require Import Vellvm.Ollvm_ast.
+Require Import Vellvm.Compiler.
+Require Import Vellvm.AstLib.
+Require Import Vellvm.CFG.
+Require Import Vellvm.StepSemantics.
+Require Import Vellvm.Memory.
 Require Import Vellvm.Classes.
 
 (* Logical Foundations dependencies *)
-Require Import Vellvm.Imp Vellvm.Maps Vellvm.ImpCEvalFun.
+Require Import Vellvm.Imp.
+Require Import Vellvm.Maps.
+Require Import Vellvm.ImpCEvalFun.
 Import ListNotations.
 
+Require Import Vellvm.ImpQuickChick.
 
 (* Equality for the imp final memory states. *)
 
 (* These definitions should probably go in a library *)
-Definition dvalue_of_nat (n:nat) : value :=
+Definition dvalue_of_nat (n:nat) : dvalue :=
   DV (VALUE_Integer (Z.of_nat n)).
 
 Definition imp_val_eqb (v1 v2 : dvalue) : bool :=
@@ -56,7 +64,7 @@ Fixpoint imp_memory_eqb (m1 : list dvalue) (m2 : list dvalue) : bool :=
 Require Import List.
 
 
-Fixpoint string_of_dvalue' (v : value) :=
+Fixpoint string_of_dvalue' (v : dvalue) :=
   match v with
   | DV expr =>
     match expr with
@@ -129,6 +137,9 @@ Definition compile_and_execute (c : Imp.com) : err mtype :=
     end
   end.
 
+
+(*! Section CompilerProp *)
+
 Definition imp_compiler_correct_aux (p:Imp.com) : Checker :=
   let fvs := IDSet.elements (fv p) in
   match compile p with
@@ -142,12 +153,12 @@ Definition imp_compiler_correct_aux (p:Imp.com) : Checker :=
       | inl e => whenFail "init failed" false
       | inr initial_state =>
         let semantics := sem mcfg initial_state in
-        let llvm_final_state := MemDFin [] semantics 10000 in
+        let llvm_final_state := MemDFin [] semantics 15000 in
         let imp_state := ceval_step empty_state p 100 in
         match (llvm_final_state, imp_state) with
         | (None, None) => whenFail "both out of gas" true
-        | (Some llvm_st, None) => whenFail "imp out of gas" true (* false *)
-        | (None, Some imp_st) => whenFail "llvm out of gas" true (* false *)
+        | (Some llvm_st, None) => whenFail "imp out of gas" true
+        | (None, Some imp_st) => whenFail "llvm out of gas" true
         | (Some llvm_st, Some imp_st) => 
           let ans_state := List.map (fun x => dvalue_of_nat (imp_st x)) fvs in
           checker (whenFail ("not equal: llvm: "
@@ -158,10 +169,199 @@ Definition imp_compiler_correct_aux (p:Imp.com) : Checker :=
                                ++ (string_of fvs) (* (elems_to_string fvs) *)
                                ++ "; compiled code: "
                                ++ (string_of ll_prog))
-                            (imp_memory_eqb (List.rev llvm_st) ans_state))
+                            (imp_memory_eqb (*!*) (List.rev llvm_st) (*! llvm_st *) ans_state))
         end        
       end
     end
   end.
 
-        
+(*
+Definition imp_compiler_correct_bool (p:Imp.com) : bool :=
+  let fvs := IDSet.elements (fv p) in
+  match compile p with
+  | inl e => false
+  | inr ll_prog =>
+    let m := modul_of_toplevel_entities ll_prog in
+    match mcfg_of_modul m with
+    | None => false
+    | Some mcfg =>
+      match init_state mcfg "imp_command" with
+      | inl e => false
+      | inr initial_state =>
+        let semantics := sem mcfg initial_state in
+        let llvm_final_state := MemDFin [] semantics 15000 in
+        let imp_state := ceval_step empty_state p 100 in
+        match (llvm_final_state, imp_state) with
+        | (None, None) => true
+        | (Some llvm_st, None) => true
+        | (None, Some imp_st) => true
+        | (Some llvm_st, Some imp_st) => 
+          let ans_state := List.map (fun x => dvalue_of_nat (imp_st x)) fvs in
+          imp_memory_eqb (List.rev llvm_st) ans_state
+        end        
+      end
+    end
+  end.
+
+
+Definition compile_aexp_bool (a:aexp) : bool :=
+  let p := (Id "fresh_var" ::= a) in
+  imp_compiler_correct_bool p.  
+
+Compute (compile_aexp_bool (AMult (ANum 2) (ANum 3))).
+*)
+
+Definition compile_aexp_correct (a:aexp) : Checker :=
+  let p := (Id "fresh_var" ::= a) in
+  imp_compiler_correct_aux p.  
+
+
+Definition compile_bexp_correct (b:bexp) : Checker :=
+  let p := (IFB b THEN idX ::= ANum 1 ELSE idY ::= ANum 2 FI) in
+  imp_compiler_correct_aux p.  
+  
+
+
+
+(* Tests *)
+
+Extract Constant Test.defNumTests => "100".
+
+(* Fails compilation because of wrongly-corrected monad_fold_left *)
+Example prog1 := (idX ::= ANum 1).
+Example prog2 := (idW ::= AId idW).
+
+(* Fails compilation because of off-by-one in Alloca for MemDFin *)
+Example prog3 := idX ::= ANum 1 ;; idY ::= ANum 2 ;; idZ ::= ANum 3 ;; idW ::= ANum 4.
+Example prog4 := idX ::= AId idY.
+Example prog5 := idX ::= APlus (AId idW) (AId idX).
+
+(* Fails compilation because of memory allocation of free vars in reverse order
+   during compilation *)
+Example prog6 := idY ::= APlus (AId idZ) (ANum 4).
+
+(* Fails because of N semantics in Imp but Z semantics for Vellvm *)
+Example prog7 :=
+  IFB (BEq (AMult (ANum 10) (AId idW)) (AMult (ANum 6) (ANum 5))) THEN
+    X ::= (APlus (AId idY) (AMult (APlus (ANum 1) (ANum 5)) (APlus (ANum 1) (ANum 0))))
+  ELSE Y ::= (APlus (AId idY) (APlus (AMinus (ANum 3) (ANum 4)) (ANum 2))) FI.
+  (* IF (10 * W == 6 * 5) THEN
+       X = Y + ( (1 + 5) * (1 + 0) )
+     ELSE
+       Y = Y + ((3 - 4) + 2)
+     END *)
+
+Example prog8 :=
+  IFB (BFalse) THEN
+    X ::= ANum 10
+  ELSE Y ::= (AMinus (ANum 3) (ANum 4)) FI.
+
+Example prog9 :=
+  Y ::= (AMinus (ANum 3) (ANum 4)).
+
+
+Definition show_aexp_compilation_result (result : err (Ollvm_ast.value * list elt)) :=
+  match result with
+  | inl _ => "err" 
+  | inr (_, elts) => string_of elts
+  end.
+
+Definition show_bexp_compilation_result (result : err (Ollvm_ast.value * list elt)) :=
+  match result with
+  | inl _ => "err"
+  | inr (_ , elts) => string_of elts
+  end.
+
+
+Definition show_result (result : err (toplevel_entities (list block))) :=
+  match result with
+  | inl _ => "error"
+  | inr l => fold_left (fun s tle_blk => (s ++ "; " ++ (string_of tle_blk))%string) l ""
+  end.
+
+(*
+Compute (show_aexp_compilation_result
+           (compile_aexp_wrapper (AMult (AId idX) (APlus (ANum 1) (ANum 2))))).
+
+Compute (show_bexp_compilation_result
+           (compile_bexp_wrapper (BEq (ANum 5) (APlus (ANum 2) (ANum 3))))).
+
+Compute (show_result (compile prog3)).
+Compute (show_result (compile prog4)).
+Compute (show_result (compile prog6)).
+
+Compute (compile_and_execute prog3).
+Compute (compile_and_execute prog4).
+Compute (compile_and_execute prog5).
+Compute (compile_and_execute prog7).
+Compute (compile_and_execute prog8).
+Compute (compile_and_execute prog9).
+*)
+
+(* Compute (compile_and_execute prog5). *)
+
+(* QuickChick (forAll arbitrary
+                   imp_compiler_correct_aux). *)
+
+(* QuickChick (forAll (test_com_gen 2) imp_compiler_correct_aux). *)
+
+
+
+(* QuickChick (forAll (test_aexp_gen) compile_aexp_correct). *)
+(* QuickChick (forAll (test_bexp_gen) compile_bexp_correct). *)
+
+
+Definition prog10 :=
+  IFB (BNot (BNot (BLe (AMult (ANum 6) (ANum 6)) (AId Y))))
+  THEN idY ::= AId idX
+  ELSE idZ ::= AId idZ FI.
+
+Definition prog11 :=
+  IFB (BLe (AMult (ANum 6) (ANum 6)) (AId Y))
+  THEN idY ::= AId idX
+  ELSE idZ ::= AId idZ FI.
+
+Definition prog12 :=
+  IFB (BNot (BNot (BLe (ANum 0) (AId Y))))
+  THEN idY ::= AId idX
+  ELSE idZ ::= AId idZ FI.
+
+Definition prog13 :=
+  IFB (BNot (BNot (BEq (ANum 0) (AId Y))))
+  THEN SKIP
+  ELSE SKIP FI.
+
+Definition prog14 :=
+  IFB (BNot (BEq (ANum 0) (AId Y)))
+  THEN SKIP
+  ELSE SKIP FI.
+
+Definition prog15 :=
+  IFB (BEq (ANum 0) (AId Y))
+  THEN SKIP
+  ELSE SKIP FI.
+
+Definition prog16 :=
+  IFB (BNot BTrue)
+  THEN SKIP
+  ELSE SKIP FI.
+
+
+(*
+Compute (show_result (compile prog10)).
+Compute (compile_and_execute prog10).
+Compute (compile_and_execute prog11).
+Compute (compile_and_execute prog12).
+Compute (compile_and_execute prog13).
+Compute (compile_and_execute prog14).
+Compute (show_result (compile prog14)).
+Compute (compile_and_execute prog15).
+Compute (compile_and_execute prog16).
+Compute (show_result (compile prog16)).
+*)
+
+(*!
+QuickChick (forAllShrink (test_com_gen 3) (@shrink com shrcom) 
+                   imp_compiler_correct_aux).
+*)
+
